Support more <<operator delete>> forms.
- `operator delete(void*)`
- `operator delete(void*, size_t)`
- `operator delete(void*, size_t, std::align_val_t)`
- `operator delete[](void*)`
- `operator delete[](void*, size_t)`
- `operator delete[](void*, size_t, std::align_val_t)`

Also contains (commented out) support for
- `T::operator delete(T*, std::destroying_delete_t)`

rocq-bluerock-brick/theories/lang/cpp/logic/new_delete.v
@@ -20,16 +20,57 @@ Require Import bluerock.lang.cpp.logic.wp.
 Require Import bluerock.lang.cpp.logic.call.
 Require Import bluerock.lang.cpp.logic.translation_unit.
 
-Require Import bedrock.lang.cpp.logic.const.
+Require Import bluerock.lang.cpp.logic.const.
 
-#[local] Notation Talign_val_t := "enum std::align_val_t"%cpp_type.
-#[local] Notation Tdestroying_delete_t := "std::destroying_delete_t"%cpp_type.
+Notation Talign_val_t := "enum std::align_val_t"%cpp_type.
+Notation Tdestroying_delete_t := "std::destroying_delete_t"%cpp_type.
 
 (* The type of the information in the AST about the default delete operator
  *)
 #[local] Notation DEFAULT_DELETE := (name)%type (only parsing).
 
 Import linearity.
+
+(* TODO: upstream? *)
+Section with_prop.
+  Context {PROP : bi}.
+  Lemma exists_frame {T} (P P' : T -> PROP) :
+    (∀ x, P x -* P' x) |-- (∃ x, P x) -* (∃ x, P' x).
+  Proof.
+    iIntros "X Y"; iDestruct "Y" as (x) "Y"; iExists x; iApply "X"; eauto.
+  Qed.
+  Lemma forall_frame {T} (P P' : T -> PROP) :
+    (∀ x, P x -* P' x) |-- (∀ x, P x) -* (∀ x, P' x).
+  Proof.
+    iIntros "X Y" (?); iApply "X"; iApply "Y".
+  Qed.
+  Lemma sep_frame (Q P P' : PROP) :
+    (P -* P') |-- (Q ** P) -* (Q ** P').
+  Proof.
+    iIntros "X [$ Y]"; iApply "X"; eauto.
+  Qed.
+  Lemma wand_frame (Q P P' : PROP) :
+    (P -* P') |-- (Q -* P) -* (Q -* P').
+  Proof.
+    iIntros "X Y Z"; iApply "X"; iApply "Y"; eauto.
+  Qed.
+End with_prop.
+Ltac do_frame :=
+  repeat match goal with
+    | |- environments.envs_entails _ ?X =>
+        match X with
+        | _ => iIntros (?)
+        | ((_ ** _) -* (_ ** _)) => iApply sep_frame
+        | ((_ -* _) -* (_ -* _)) => iApply wand_frame
+        | ((bi_forall _) -* (bi_forall _)) => iApply forall_frame; iIntros (?)
+        | ((bi_exist _) -* (bi_exist _)) => iApply exists_frame; iIntros (?)
+        | _ => iApply wp_fptr_frame; iIntros (?)
+        | _ => iApply interp_frame
+        | _ => iApply operand_receive_frame
+        end; eauto
+    end.
+(* END: upstream *)
+
 
 (* TODO: refactor this *)
 Module delete_operator.
@@ -59,15 +100,18 @@ Module delete_operator.
     in
     Tfunction (FunctionType Tvoid args).
 
+  #[local]
   Definition get_destroying {T} (k : list type -> option T) (args : list type) : option (option name * T) :=
     match args with
     | Tptr (Tnamed nm) :: t :: rest =>
         let is_destroying_delete_t t := bool_decide (t = Tdestroying_delete_t) in
         if is_destroying_delete_t t then
           pair (Some nm) <$> k rest
-        else pair None <$> k args
-    | _ => pair None <$> k args
+        else None
+    | Tptr Tvoid :: rest => pair None <$> k rest
+    | _ => None
     end.
+  #[local]
   Definition get_size_t {T} (k : list type -> option T) (args : list type) : option (bool * T) :=
     match args with
     | t :: rest =>
@@ -76,6 +120,7 @@ Module delete_operator.
         else pair false <$> k args
     | _ => pair false <$> k args
     end.
+  #[local]
   Definition get_align_t {T} (k : list type -> option T) (args : list type) : option (bool * T) :=
     match args with
     | t :: rest =>
@@ -85,6 +130,8 @@ Module delete_operator.
     | _ => pair false <$> k args
     end.
 
+  (** Given the type of an <<operator delete>> (or <<operator delete[]>>) type,
+      determine the information that it needs to be invoked with *)
   Definition classify (ty : type) : option delete_operator.t :=
     match ty with
     | Tfunction ft =>
@@ -96,6 +143,78 @@ Module delete_operator.
         else None
     | _ => None
     end.
+
+  #[local] Definition with_delete (tu : translation_unit) (nm : obj_name)
+    : option (obj_name * delete_operator.t) :=
+    pair nm <$> (tu.(symbols) !! nm >>= fun del_fn => delete_operator.classify (type_of_value del_fn)).
+
+  #[local] Definition delete_for_named (tu : translation_unit) (default_delete : DEFAULT_DELETE)
+    (cls : name) : option (obj_name * delete_operator.t) :=
+    match tu.(types) !! cls with
+    | Some (Gstruct s) =>
+        with_delete tu $ stdpp.option.default default_delete s.(s_delete)
+    | Some (Gunion u) =>
+        with_delete tu $ stdpp.option.default default_delete u.(u_delete)
+    | Some (Genum _ _) =>
+        with_delete tu default_delete
+    | _ => None
+    end.
+
+  (** The <<operator delete>> that is used when deleting a **complete object**
+      of type <<ty>>. [default] is the default delete operator used to delete
+      the object if there is no type-specific override, e.g.
+      <<T::operator delete(...)>>.
+
+      To delete an array of type <<ety>>, <<ty>> should be <<Tincomplete_array ety>>.
+   *)
+  Definition delete_for (tu : translation_unit) (default_delete : DEFAULT_DELETE) (ty : type)
+    : option (obj_name * delete_operator.t) :=
+    match erase_qualifiers ty with
+    | Tnamed cls => delete_for_named tu default_delete cls
+    | Tincomplete_array _
+    | Tarray _ _ => with_delete tu default_delete
+    | Tvariable_array _ _ => None
+    | _ => with_delete tu default_delete
+    end.
+
+  #[local]
+  Lemma with_delete_sub_module {tu1 tu2 nm result} :
+    with_delete tu1 nm = Some result ->
+    sub_module tu1 tu2 ->
+    with_delete tu2 nm = Some result.
+  Proof.
+    rewrite /with_delete; intros.
+    destruct (symbols tu1 !! nm) eqn:Heq; simpl in *; try congruence.
+    destruct H0. edestruct syms_compat. eassumption.
+    destruct H0 as [HH Hle]. rewrite HH /=.
+    erewrite <-type_of_value_ObjValue_ler; eauto.
+  Qed.
+
+  #[local]
+  Lemma delete_for_named_sub_module {tu1 tu2 def cls result} :
+    delete_for_named tu1 def cls = Some result ->
+    sub_module tu1 tu2 ->
+    delete_for_named tu2 def cls = Some result.
+  Proof.
+    rewrite /delete_for_named; intros.
+    destruct (types tu1 !! cls) eqn:Heq; simpl in *; try congruence.
+    destruct g; try congruence.
+    { erewrite sub_module_preserves_gunion; eauto using with_delete_sub_module. }
+    { erewrite sub_module_preserves_gstruct; eauto using with_delete_sub_module. }
+    { edestruct sub_module_preserves_genum; eauto.
+      rewrite H1. eauto using with_delete_sub_module. }
+  Qed.
+
+  Lemma delete_for_submodule {tu1 tu2 op cls result} :
+    delete_for tu1 op cls = Some result ->
+    sub_module tu1 tu2 ->
+    delete_for tu2 op cls = Some result.
+  Proof.
+    rewrite /delete_for.
+    intros.
+    repeat (case_match; eauto using with_delete_sub_module, delete_for_named_sub_module).
+  Qed.
+
 End delete_operator.
 (* END: refactor this *)
 
@@ -456,114 +575,113 @@ Module Type Expr__newdelete.
       End new.
     End with_region.
 
-    (** *** [wp_delete] *)
-    Definition alloc_pointer (pv : ptr) (Q : ptr -> FreeTemp -> mpred) : mpred :=
-      Forall p : ptr, p |-> primR (Tptr Tvoid) 1$m (Vptr pv) -* Q p (FreeTemps.delete (Tptr Tvoid) p).
+  End with_cpp_logic.
 
-    Lemma alloc_pointer_frame : forall p Q Q',
-        Forall p fr, Q p fr -* Q' p fr |-- alloc_pointer p Q -* alloc_pointer p Q'.
-    Proof.
-      intros; rewrite /alloc_pointer. iIntros "X Y".
-      iIntros (?) "p"; iApply "X"; iApply "Y"; done.
-    Qed.
+  (** ** <<delete>> and <<delete[]>> *)
 
-    (** [resolve_dtor ty obj_ptr' Q] resolves the destructor for the object [obj_ptr'] (of type [ty]).
-        The continuation [Q] is passed the pointer to the most-derived-object of [obj_ptr] and its type.
+  (** [resolve_complete_obj ty obj_ptr' Q] resolves the destructor for the object
+      <<obj_ptr'>> (of type <<ty>>). The continuation [Q] is passed the pointer to the
+      most-derived-object of <<obj_ptr>> and its type.
 
-        NOTE: This only resolves the complete object if the destructor is <<virtual>>. Otherwise,
-              the class itself is returned.
-      *)
-    Definition resolve_complete_obj (tu : translation_unit) (ty : type) (obj_ptr' : ptr) (Q : ptr -> type -> mpred) : mpred :=
-      match drop_qualifiers ty with
-      | Tqualified _ ty => False (* unreachable *)
-      | Tnamed cls      =>
-        match tu.(types) !! cls with
-        | Some (Gstruct s) =>
-          if has_virtual_dtor s then
-            (* NOTE [has_virtual_dtor] could be derived from the vtable... *)
-            (* In this case, use virtual dispatch to invoke the destructor. *)
-            letI* fimpl, impl_class, obj_ptr := resolve_virtual obj_ptr' cls s.(s_dtor) in
-            let r_ty := Tnamed impl_class in
-            Q obj_ptr r_ty
-          else
-            Q obj_ptr' (erase_qualifiers ty)
-        | Some (Gunion u)  =>
-          (* Unions cannot have [virtual] destructors: we directly invoke the destructor. *)
+      NOTE: This only resolves the complete object if the destructor is <<virtual>>.
+            Otherwise, the class itself is returned.
+
+      NOTE: The implementation does **not** take the current translation unit
+            and instead looks up the class in the ambient (global) program. By the
+            one-definition-rule (ODR), looking up the result in the whole program will
+            yield an answer that is at least as informative as one that looks up
+            in the current translation unit. So if the dispatch is <<virtual>> in
+            the whole program, then the dispatch must also be <<virtual>> in the
+            local translation unit (as long as the program is well-typed).
+
+      NOTE: <<erase_qualifiers>> is probably not necessary here.
+    *)
+  mlock
+  Definition resolve_complete_obj `{Σ : cpp_logic} {σ : genv} (ty : type)
+    (obj_ptr' : ptr) (Q : ptr -> type -> mpred) : mpred :=
+    match drop_qualifiers ty with
+    | Tqualified _ ty => False (* unreachable *)
+    | Tnamed cls      =>
+      match (genv_tu σ).(types) !! cls with
+      | Some (Gstruct s) =>
+        if has_virtual_dtor s then
+          (* NOTE [has_virtual_dtor] could be derived from the vtable... *)
+          (* In this case, use virtual dispatch to invoke the destructor. *)
+          letI* fimpl, impl_class, obj_ptr := resolve_virtual obj_ptr' cls s.(s_dtor) in
+          let r_ty := Tnamed impl_class in
+          Q obj_ptr r_ty
+        else
           Q obj_ptr' (erase_qualifiers ty)
-        | _                => False
-        end
-      | Tarray _ _
-      | Tincomplete_array _
-      | Tvariable_array _ _ =>
+      | Some (Gunion u)  =>
+        (* Unions cannot have [virtual] destructors: we directly invoke the destructor. *)
         Q obj_ptr' (erase_qualifiers ty)
-      | Tref r_ty
-      | Trv_ref r_ty    =>
-        False (* references can not be deleted, only destroyed *)
-      | ty              =>
+      | Some (Genum _ _) =>
         Q obj_ptr' (erase_qualifiers ty)
-      end%I.
+      | _                => False
+      end
+    | Tarray _ _
+    | Tincomplete_array _
+    | Tvariable_array _ _ =>
+      Q obj_ptr' (erase_qualifiers ty)
+    | Tref r_ty
+    | Trv_ref r_ty    =>
+      False (* references can not be deleted, only destroyed *)
+    | ty              =>
+      Q obj_ptr' (erase_qualifiers ty)
+    end%I.
 
-    Lemma resolve_complete_obj_frame : forall tu ty p Q Q',
-        Forall p t, Q p t -* Q' p t |-- resolve_complete_obj tu ty p Q -* resolve_complete_obj tu ty p Q'.
+  Section with_cpp.
+    Context `{Σ : cpp_logic} {σ : genv}.
+    Lemma resolve_complete_obj_frame : forall ty p Q Q',
+        Forall p t, Q p t -* Q' p t |-- resolve_complete_obj ty p Q -* resolve_complete_obj ty p Q'.
     Proof.
-      rewrite /resolve_complete_obj; intros.
+      rewrite resolve_complete_obj.unlock; intros.
       iIntros "X"; repeat case_match; eauto; try solve [ iApply wp_fptr_frame; iIntros (?); eauto ].
       iApply resolve_virtual_frame. iIntros (???); iApply "X".
     Qed.
 
-    Definition cv_compat (t1 t2 : type) : Prop :=
-      erase_qualifiers t1 = erase_qualifiers t2.
+    (** [delete_compat dealloc alloc] holds when the allocation type <<alloc>>
+        can be deleted by an expression representing the deallocation type
+        <<dealloc>>.
 
-    Lemma cv_compat_refl ty :
-      cv_compat ty ty.
-    Proof. done. Qed.
+        Normally, this means that <<dealloc = alloc>>, but we use
+        [Tincomplete_array] to approximate any array type, therefore we can
+        [delete_compat (Tincomplete_array ety) (Tarray ety _)] holds.
 
-  End with_cpp_logic.
+        Importantly, when we check this in the case of <<virtual>> dispatch,
+        <<dealloc>> will be the type of the complete object, **not** the type
+        of the pointer used to perform the <<delete>>. These types are guaranteed
+        to be related because we compute the type of the complete object through
+        [resolve_complete_obj] which uses [derivationR].
+     *)
+    Definition delete_compat (dealloc_type alloc_type : type) : Prop :=
+      match erase_qualifiers dealloc_type , erase_qualifiers alloc_type with
+      | Tincomplete_array ety , Tarray ety' _ => ety = ety'
+      | dealloc , alloc => dealloc = alloc
+      end.
 
-  (** [array_compatible true ty] holds when [ty] is an array type that can
-      be <<new>>d.
-      [array_compatible false ty] holds when [ty] is **not** an array type.
+    #[global] Instance delete_compat_dec {dealloc alloc}
+      : Decision (delete_compat dealloc alloc) :=
+      ltac:(rewrite /delete_compat; repeat case_match; apply _).
+
+    Lemma delete_compat_refl ty : delete_compat ty ty.
+    Proof. rewrite /delete_compat. destruct (erase_qualifiers ty); simpl; eauto. Qed.
+  End with_cpp.
+
+  (** Invoke the delete operator <<del_op.1>> on the pointer <<p>> for the type
+      <<obj_type>>. The type <<obj_type>> is used to get the size and
+      alignedness information if the <<operator delete>> requires them.
+
+      NOTE: <<p>> should be the object pointer in the case of destroying delete
+            and otherwise should be the storage pointer.
+
+      NOTE: <<allocation_size>> must be the size of the entire allocation
+            (including overhead). This is especially relevant when deleting
+            an array.
    *)
-  Definition array_compatible (is_array : bool) (ty : type) : Prop :=
-    match ty with
-    | Tarray _ _ => is_array = true
-    | Tincomplete_array _
-    | Tvariable_array _ _ => False
-    | _ => is_array = false
-    end.
-
-  (** The <<operator delete>> that is used when deleting a **complete object** of type <<ty>>.
-     [default] is the default delete operator used to delete the object if there is no
-     type-specific override, e.g. <<T::operator delete(...)>>.
-   *)
-  Definition delete_for (array : bool) (tu : translation_unit) (default_delete : DEFAULT_DELETE) (ty : type)
-    : option (obj_name * delete_operator.t) :=
-    let del_of_name nm :=
-      pair nm <$> (tu.(symbols) !! nm >>= fun del_fn => delete_operator.classify (type_of_value del_fn))
-    in
-    match erase_qualifiers ty with
-    | Tnamed cls =>
-        match tu.(types) !! cls with
-        | Some (Gstruct s) =>
-            del_of_name $ default default_delete s.(s_delete)
-        | Some (Gunion u) =>
-            del_of_name $ default default_delete u.(u_delete)
-        | Some (Genum _ _) =>
-            del_of_name default_delete
-        | _ => None
-        end
-    | _ => del_of_name default_delete
-    end.
-
-  (** Invoke the delete operator <<del_op.1>> on the pointer <<p>> for the type <<obj_type>>.
-      The type <<obj_type>> is used to get the size and alignedness information if the
-      <<operator delete>> requires them.
-
-      NOTE: <<p>> should be the object pointer in the case of destroying delete and otherwise
-      should be the storage pointer.
-   *)
-  Definition wp_invoke_delete `{Σ : cpp_logic} {σ : genv} (tu : translation_unit) (obj_type : type)
-    (del_op : name * delete_operator.t)
+  mlock
+  Definition wp_invoke_delete `{Σ : cpp_logic} {σ : genv} (obj_type : type)
+    (del_op : name * delete_operator.t) (allocation_size : N)
     (p : ptr) (Q : mpred) : mpred :=
     letI* args , free := fun (Q : list ptr -> FreeTemps.t -> mpred) =>
         (* Add the alignment, if required *)
@@ -577,20 +695,24 @@ Module Type Expr__newdelete.
       (* Add the size, if required *)
       if del_op.2.(delete_operator.size_arg) then
          let ty := Tsize_t in
-         Exists sz, [| size_of obj_type = Some sz |] **
-         Forall pp : ptr, pp |-> primR ty (cQp.m 1) (Vn sz) -* Q (pp :: args) (FreeTemps.delete ty pp >*> free)
+         Forall pp : ptr, pp |-> primR ty (cQp.m 1) (Vn allocation_size) -* Q (pp :: args) (FreeTemps.delete ty pp >*> free)
       else Q args free
     in
     letI* args , free := fun (Q : list ptr -> FreeTemps.t -> mpred) =>
       (* Add the pointer (and the <<std::destroying_delete_t>> flag if necessary) *)
       if del_op.2.(delete_operator.destroying) then
-        (* In addition to the pointer, we must also pass the value of type <<std::destroying_delete_t>>.
-           This value is passed by-value, which means that it is copied. The implementation is just a marker,
-           so the only ownership is the <<structR>> ownership.
+        (* In addition to the pointer, we must also pass the value of type
+           <<std::destroying_delete_t>>. This value is passed by-value, which means
+           that it is copied. Here we assume the following implementation:
+           <<
+           struct std::destroying_delete_t {};
+           >>
+           We capture the ownership using [anyR "std::destroying_delete_t" (cQp.m 1)]
+           but we could also check that the structure exists.
          *)
         let ty := erase_qualifiers $ Tptr obj_type in
         Forall pp : ptr, pp |-> primR ty (cQp.m 1) (Vptr p) -*
-        Forall dd : ptr, dd |-> structR "std::destroying_delete_t" (cQp.m 1) -*
+        Forall dd : ptr, dd |-> anyR "std::destroying_delete_t" (cQp.m 1) -*
         Q (pp :: dd :: args) (FreeTemps.delete ty pp >*> FreeTemps.delete Tdestroying_delete_t dd >*> free)
       else
         let ty := "void*"%cpp_type in
@@ -599,10 +721,21 @@ Module Type Expr__newdelete.
     in
     letI* p :=
       let del_ty := delete_operator.type_for del_op.2 in
-      wp_fptr tu.(types) del_ty (_global del_op.1) args in
-    letI* := interp tu free in
+      wp_fptr (genv_tu σ).(types) del_ty (_global del_op.1) args in
+    letI* := interp (genv_tu σ) free in
     letI* _ := operand_receive "void" p in
     Q.
+
+  Lemma wp_invoke_delete_frame `{Σ : cpp_logic} {σ : genv}
+    obj_type operator_delete size obj_ptr Q Q' :
+    Q -* Q'
+    |-- wp_invoke_delete obj_type operator_delete size obj_ptr Q -*
+        wp_invoke_delete obj_type operator_delete size obj_ptr Q'.
+  Proof.
+    rewrite wp_invoke_delete.unlock.
+    iIntros "H";
+    repeat case_match; simpl; do_frame.
+  Qed.
 
   (** [wp_delete_null]
       The semantics of <<delete static_cast<destroyed_type*>(nullptr);>>
@@ -611,33 +744,83 @@ Module Type Expr__newdelete.
       <<operator delete>> or to do nothing. To support this, the semantics
       uses a classical conjunction to represent non-deterministic (demonic)
       choice.
+
+      NOTE: As with [wp_delete_obj], to invoke <<delete[]>>, [destroyed_type]
+      should be [Tincomplete_array element_type].
    *)
-  Definition wp_delete_null `{Σ : cpp_logic} {σ : genv} tu (array : bool)
+  mlock
+  Definition wp_delete_null `{Σ : cpp_logic} {σ : genv}
     default_delete destroyed_type Q : mpred :=
-    match delete_for array tu default_delete destroyed_type with
-    | Some del_op => wp_invoke_delete tu destroyed_type del_op nullptr Q
-    | None => False
-    end ∧ Q.
+    (match delete_operator.delete_for (genv_tu σ) default_delete destroyed_type with
+     | Some del_op =>
+         (* The use of <<0>> here is somewhat arbitrary. It is supposed to be
+            the size of the allocation (including overhead). For deleting
+            <<nullptr>>, there is no object, but the standard does say that
+            it is legal to call this function. In practice, it seems
+            like compilers do not do this.
+          *)
+         wp_invoke_delete destroyed_type del_op 0 nullptr Q
+     | None => False
+     end ∧ Q).
+
+  Lemma wp_delete_null_frame `{Σ : cpp_logic} {σ : genv}
+    default_delete destroyed_type Q Q' :
+    Q -* Q'
+    |-- wp_delete_null default_delete destroyed_type Q -*
+        wp_delete_null default_delete destroyed_type Q'.
+  Proof.
+    rewrite wp_delete_null.unlock.
+    case_match; do_frame.
+    { iIntros "H"; do_frame.
+      iIntros "H'"; iSplit.
+      - by iDestruct "H'" as "[H' _]"; iRevert "H'"; iApply wp_invoke_delete_frame.
+      - iDestruct "H'" as "[_ H']"; iApply "H"; eauto. }
+    { iIntros "H"; do_frame; iIntros "X"; iSplit.
+      iDestruct "X" as "[[] _]".
+      iDestruct "X" as "[_ X]"; iApply "H"; eauto. }
+  Qed.
 
   (** [wp_delete_obj tu obj_type d obj_ptr storage_ptr Q]
       Delete the object [obj_ptr] (of C++ type <<obj_type>>) that occupies the storage [storage_ptr].
       [obj_ptr] should be the pointer to the complete object meaning that no virtual dispatch occurs
       here.
+
+      This weakest pre-condition does **not** take a translation unit because object deletion is
+      (effectively) handled by 0-argument closures. For example, suppose that you have the following
+      program:
+      <<
+      // header.hpp
+      struct C { virtual ~C() = 0; };
+
+      void delete_it(C* p) { delete p; }
+
+      // impl.cpp
+      struct D : C { operator delete(D*, std::destroying_delete_t) { ... } };
+
+      void test() { delete_it(new D()); }
+      >>
+
+      In this case, <<delete_it>> ultimately invokes <<D::operator delete(D*, std::destroying_delete_t)>>
+      but the implementation of <<delete_it>> can not see that function statically.
    *)
-  Definition wp_delete_obj `{Σ : cpp_logic} {σ : genv} (array : bool) (tu : translation_unit)
+  mlock
+  Definition wp_delete_obj `{Σ : cpp_logic} {σ : genv}
     (default_delete : DEFAULT_DELETE) (obj_type : type)
     (obj_ptr : ptr) (Q : mpred) : mpred :=
-    match delete_for false tu default_delete obj_type with
+    match delete_operator.delete_for (genv_tu σ) default_delete obj_type with
     | None => ERROR ("wp_delete_obj: failed to find <<operator delete>> for type"%pstring, obj_type)
     | Some del_op =>
-      Exists cv_type storage_ptr overhead sz,
-        obj_ptr |-> new_token.R 1 (new_token.mk cv_type storage_ptr overhead) ** [| cv_compat cv_type obj_type |] **
-        [| size_of cv_type = Some sz |] **
+      Exists alloc_type storage_ptr overhead sz,
+        obj_ptr |-> new_token.R 1 (new_token.mk alloc_type storage_ptr overhead) **
+        [| delete_compat obj_type alloc_type |] **
+        [| size_of alloc_type = Some sz |] **
         if del_op.2.(delete_operator.destroying) is Some _ then
-          let '(cv, ty) := decompose_type cv_type in
+          UNSUPPORTED ("wp_delete_obj: destroying delete is not supported"%pstring, obj_type)
+          (* Sketch implementation. Test cases needed.
+          let '(cv, ty) := decompose_type alloc_type in
           letI* :=
             if q_const cv
-            then wp_make_mutable tu obj_ptr ty
+            then wp_make_mutable (genv_tu σ) obj_ptr ty
             else (fun Q => Q)
           in
           (* This magic wand gives the destroying <<operator delete>> the ability
@@ -645,62 +828,52 @@ Module Type Expr__newdelete.
              at the storage pointer. The use of <<K>> requires (meta-theoretically)
              that the destruction of the object occurs within the implementation of
              the <<operator delete>>.
+
+             Note that there is no destroying delete operator for arrays, so, in
+             practice we know that <<overhead = 0>> here. In practice, a specification
+             for a destroying delete operator would look like the following:
+             [[
+             \arg{p} "p" (Vptr p)
+             \arg{delp} "" (Vptr delp)
+             \pre p |-> R (cQp.m 1) ...
+             \pre{storage_ptr K}
+                (p |-> tblockR T (cQp.m 1) -* |={top}=>
+                 storage_ptr |-> blockR (size_of T) (cQp.m 1) ** K)
+             \persist provides_storage storage_ptr p
+             \post K
+             ]]
+             Note that the implementation would be required to use <<std::launder>>
+             in order to get <<storage_ptr>> from <<obj_ptr>>.
            *)
           Forall K,
            (obj_ptr |-> tblockR (erase_qualifiers obj_type) (cQp.m 1) -* |={top}=>
             storage_ptr .[ Tuchar ! -overhead ] |-> blockR (overhead + sz) (cQp.m 1) ** K) -*
-           letI* := wp_invoke_delete tu ty del_op obj_ptr in
+           letI* := wp_invoke_delete ty del_op (overhead + sz) obj_ptr in
            K ** Q
+           *)
         else
-          letI* := interp tu (FreeTemps.delete cv_type obj_ptr) in
-          [| array_compatible array cv_type |] **
+          letI* := interp (genv_tu σ) (FreeTemps.delete alloc_type obj_ptr) in
           (storage_ptr .[ Tuchar ! -overhead ] |-> blockR (overhead + sz) (cQp.m 1) -*
            (* the <<operator delete>> is invoked with the beginning of the storage pointer *)
-           letI* := wp_invoke_delete tu obj_type del_op (storage_ptr .[ Tbyte ! -overhead ]) in
+           letI* := wp_invoke_delete obj_type del_op (overhead + sz) (storage_ptr .[ Tbyte ! -overhead ]) in
            Q)
     end%I.
 
-  (*
-  Lemma delete_val_frame `{Σ : cpp_logic} {σ : genv} : forall tu default ty p Q Q',
-      Q -* Q' |-- delete_val tu default ty p Q -* delete_val tu default ty p Q'.
+  Lemma wp_delete_obj_frame `{Σ : cpp_logic} {σ : genv}
+    default_delete destroyed_type p Q Q' :
+    Q -* Q'
+    |-- wp_delete_obj default_delete destroyed_type p Q -*
+        wp_delete_obj default_delete destroyed_type p Q'.
   Proof.
-    rewrite delete_val.unlock; intros.
-    iIntros "X"; repeat case_match; eauto; iApply alloc_pointer_frame; iIntros (??);
-    iIntros "Y !>"; iRevert "Y";
-    iApply wp_fptr_frame; iIntros (?); iApply interp_frame; iApply operand_receive_frame; iIntros (?); done.
+    rewrite wp_delete_obj.unlock.
+    iIntros "H";
+      repeat first [ case_match | progress do_frame ].
+    - iIntros "[]".
+      (* iApply wp_const_frame; first reflexivity.
+      do_frame. iApply wp_invoke_delete_frame. do_frame. *)
+    - iApply wp_invoke_delete_frame; do_frame; eauto.
+    - iIntros "[]".
   Qed.
-  *)
-
-  (*
-  (* [wp_delete] encapsulates the logic needed to <<delete>> an
-      object of a particular type.
-    *)
-  mlock
-  Definition wp_delete `{Σ : cpp_logic} {σ : genv} (tu : translation_unit)
-    (default_delete : obj_name * type) (destroyed_type : type)
-    (obj_ptr : ptr) (Q : mpred) : mpred :=
-    denoteModule tu -*
-    ()%I.
-  #[global] Arguments wp_delete {_ _ _ σ}.
-
-  Definition wp_delete_array `{Σ : cpp_logic} {σ : genv} (tu : translation_unit)
-    (default_delete : obj_name * type) (destroyed_type : type)
-    (obj_ptr : ptr) (Q : mpred) : mpred :=
-    denoteModule tu -*
-      (if bool_decide (obj_ptr = nullptr)
-       then
-         (* this conjunction justifies the compiler calling the delete function
-         or not calling it when the argument is null. *)
-         (match delete_for true tu default_delete destroyed_type with
-          | Some del_op => wp_do_delete tu del_op destroyed_type obj_ptr Q
-          | None => False
-          end)
-         ∧ Q
-       else
-         (* There is not <<virtual>> dispatch for <<delete[]>> *)
-         wp_delete_obj true tu default_delete destroyed_type obj_ptr Q)%I.
-  #[global] Arguments wp_delete_array {_ _ _ σ}.
-  *)
 
   Section delete.
     Context `{Σ : cpp_logic} {σ : genv}.
@@ -709,29 +882,6 @@ Module Type Expr__newdelete.
       Variable (tu : translation_unit).
       Context (ρ : region).
       #[local] Notation wp_operand := (wp_operand tu ρ).
-
-      (*
-      Lemma wp_delete_frame : forall tu fn ary ty p Q Q',
-          Q -* Q' |-- wp_delete tu fn ty ary p Q -* wp_delete tu fn ty ary p Q'.
-      Proof.
-        rewrite wp_delete.unlock; intros.
-        iIntros "X Y M"; iSpecialize ("Y" with "M"); iRevert "Y".
-        case_bool_decide.
-        { iIntros "Y"; iSplit;
-            [ iDestruct "Y" as "[Y _]"; iRevert "Y"; iApply delete_val_frame; done
-            | iDestruct "Y" as "[_ Y]"; iApply "X"; iApply "Y" ]. }
-        { iApply resolve_dtor_frame; iIntros (??) "Y".
-          iDestruct "Y" as (???) "Y".
-          iExists _, _, _.
-          iDestruct "Y" as "[$[$[$Y]]]".
-          iDestruct "Y" as (?) "Y".
-          iExists _; iDestruct "Y" as "[$ Y]".
-          iRevert "Y"; iApply destroy_val_frame; first reflexivity.
-          iIntros "Y"; iDestruct "Y" as (?) "Y"; iExists _; iDestruct "Y" as "[$ Y]".
-          iIntros "Z"; iSpecialize ("Y" with "Z").
-          iRevert "Y"; iApply delete_val_frame. eauto. }
-      Qed.
-        *)
 
       (* <<delete>>
 
@@ -760,11 +910,10 @@ Module Type Expr__newdelete.
         (letI* v , free := wp_operand e in
          Exists obj_ptr, [| v = Vptr obj_ptr |] **
          if bool_decide (obj_ptr = nullptr) then
-           wp_delete_null tu false default_delete destroyed_type (Q Vvoid free)
+           wp_delete_null default_delete destroyed_type (Q Vvoid free)
          else
-           letI* this', mdc_ty := resolve_complete_obj tu destroyed_type obj_ptr in
-           Exists tu', denoteModule tu' **
-                       wp_delete_obj false tu' default_delete mdc_ty obj_ptr (Q Vvoid free))
+           letI* this', mdc_ty := resolve_complete_obj destroyed_type obj_ptr in
+           wp_delete_obj default_delete mdc_ty this' (Q Vvoid free))
       |-- wp_operand (Edelete false default_delete e destroyed_type) Q.
 
       (** [wp_operand_delete_default] specializes [wp_operand_delete] for invocations of
@@ -775,9 +924,8 @@ Module Type Expr__newdelete.
         (* call the destructor on the object, and then call delete_fn *)
         (letI* v, free := wp_operand e in
          Exists obj_ptr, [| v = Vptr obj_ptr |] ** [| obj_ptr <> nullptr |] **
-           letI* this', mdc_ty := resolve_complete_obj tu destroyed_type obj_ptr in
-           Exists tu', denoteModule tu' **
-                       wp_delete_obj false tu' default_delete mdc_ty obj_ptr (Q Vvoid free))
+           letI* this', mdc_ty := resolve_complete_obj destroyed_type obj_ptr in
+           wp_delete_obj default_delete mdc_ty this' (Q Vvoid free))
       |-- wp_operand (Edelete false default_delete e destroyed_type) Q.
       Proof.
         intros **; iIntros "operand".
@@ -789,17 +937,15 @@ Module Type Expr__newdelete.
         case_bool_decide; try congruence; eauto.
       Qed.
 
-      (* NOTE: [destroyed_type] will refer to the /element/ of the array *)
+      (* NOTE: <<destroyed_type>> will refer to the /element/ of the array *)
       Axiom wp_operand_array_delete : forall default_delete e destroyed_type Q,
         (* call the destructor on the object, and then call delete_fn *)
         (letI* v, free := wp_operand e in
          Exists obj_ptr, [| v = Vptr obj_ptr |] **
          if bool_decide (obj_ptr = nullptr) then
-           wp_delete_null tu false default_delete destroyed_type (Q Vvoid free)
+           wp_delete_null default_delete (Tincomplete_array destroyed_type) (Q Vvoid free)
          else
-           Exists array_size,
-           let array_type := Tarray destroyed_type array_size in
-           wp_delete_obj true tu default_delete array_type obj_ptr (Q Vvoid free))
+           wp_delete_obj default_delete (Tincomplete_array destroyed_type) obj_ptr (Q Vvoid free))
       |-- wp_operand (Edelete true default_delete e destroyed_type) Q.
 
       Section NOTE_potentially_relaxing_array_delete.
